platform/cito/CModule.v
@@ -1,0 +1,51 @@
+Set Implicit Arguments.
+
+Require Import GoodModuleDec.
+Require Import FuncCore.
+
+Record CFun :=
+  {
+    Core : FuncCore;
+    good_func : is_good_func Core = true
+  }.
+    
+Coercion Core : CFun >-> FuncCore.
+
+Require Import StringMap.
+
+Record CModule := 
+  {
+    Funs : StringMap.t CFun
+  }.
+
+Require Import GoodModuleDec.
+Require Import GoodModule.
+Require Import GoodFunction.
+
+Definition cfun_to_gfun (name : string) (f : CFun) : GoodFunction.
+  refine (Build_GoodFunction (Build_Func name f) _).
+  destruct f; simpl in *.
+  eapply is_good_func_sound; eauto.
+Defined.
+
+Require Import StringMap.
+Require Import StringMapFacts.
+
+Definition cfuns_to_gfuns (fs : StringMap.t CFun) : list GoodFunction := List.map (uncurry cfun_to_gfun) (StringMap.elements fs).
+
+Require Import NameDecoration.
+
+Lemma cfuns_to_gfuns_nodup fs : NoDup (List.map (fun (f : GoodFunction) => SyntaxFunc.Name f) (cfuns_to_gfuns fs)).
+Proof.
+  unfold cfuns_to_gfuns.
+  rewrite map_map.
+  simpl.
+  eapply NoDup_elements; eauto.
+Qed.
+
+Definition cmodule_to_gmodule name (H : is_good_module_name name = true) (m : CModule) : GoodModule.GoodModule.
+  refine (@Build_GoodModule name _ (cfuns_to_gfuns (Funs m)) _).
+  eapply is_good_module_name_sound; eauto.
+  eapply cfuns_to_gfuns_nodup.
+Defined.
+
