platform/facade/CompileModule.v
@@ -3,79 +3,35 @@ Set Implicit Arguments.
 Require Import FModule.
 Require Import Compile.
 Require Import Facade.
-Require Import GoodFunction.
-Require Import GoodModule.
-Require Import NameDecoration.
 
 Section ADTValue.
 
   Variable ADTValue : Type.
 
-  Notation FModule := (@FModule ADTValue).
-
-  Require Import String.
-  Local Open Scope string_scope.
-
-  Variable m_name : string.
-
-  Hypothesis good_name : is_good_module_name m_name = true.
-
-  Variable module : FModule.
+  Variable module : FModule ADTValue.
 
   Notation FName := SyntaxFunc.Name.
   Notation MName := GoodModule.Name.
 
-  Require Import GoodFunc.
+  Require Import CModule.
   Require Import Semantics.
-  Require Import GoodModuleDec.
 
-  Lemma compile_GoodFunc (f : FFunction) : GoodFunc (compile_op f).
-  Proof.
-    destruct f; simpl in *.
-    eapply is_good_func_sound; eauto.
-  Qed.
-
-  Definition compile_func (name : string) (f : FFunction) : GoodFunction.
-    refine
-      ({|
-          GoodFunction.Fun := 
-            {|
-              SyntaxFunc.Name := name;
-              SyntaxFunc.Core := compile_op f
-            |};
-          IsGoodFunc := _
-        |}).
-    simpl.
-    eapply compile_GoodFunc.
-  Defined.
+  Definition compile_func (f : FFunction) : CFun := Build_CFun (compile_op f) (syntax_ok f).
 
   Require Import StringMap.
   Import StringMap.
   Require Import StringMapFacts.
 
-  Definition compile_funcs (funs : StringMap.t FFunction) := List.map (uncurry compile_func) (elements funs).
+  Definition compile_to_cmodule : CModule := Build_CModule (StringMap.map compile_func (FModule.Functions module)).
 
-  Lemma NoDup_elements elt (m : StringMap.t elt) : NoDup (List.map fst (elements m)).
-  Proof.
-    eapply NoDupKey_NoDup_fst.
-    eapply elements_3w.
-  Qed.
+  Require Import String.
 
-  Definition compile : GoodModule.
-    refine 
-      ({|
-          Name := m_name;
-          GoodModuleName := _;
-          Functions := compile_funcs (FModule.Functions module);
-          NoDupFuncNames := _
-        |}).
-    eapply is_good_module_name_sound; eauto.
-    unfold compile_funcs.
-    unfold uncurry.
-    rewrite map_map.
-    unfold compile_func.
-    simpl.
-    eapply NoDup_elements.
-  Defined.
+  Variable name : string.
+
+  Require Import NameDecoration.
+
+  Hypothesis good_name : is_good_module_name name = true.
+
+  Definition compile_to_gmodule : GoodModule.GoodModule := cmodule_to_gmodule name good_name compile_to_cmodule.
 
 End ADTValue.
